Implemented ECDHE and FFDHE functions in HSCrypto

src/tls/DHGroup.fst
@@ -1,81 +1,76 @@
 ﻿module DHGroup
 
+open FStar.HyperHeap
 open Platform.Bytes
 open Platform.Error
-open TLSError
 open CoreCrypto
-open FStar.HyperHeap
+open TLSError
+open TLSConstants
 
+type params = dhp:CoreCrypto.dh_params{length dhp.dh_p < 65536 && length dhp.dh_g < 65536}
 
-type elt = bytes
+type share = b:bytes{length b < 65536}
 
-(* Use to idealize *)
-type preds = | Elt of bytes * bytes * elt
-type predPP = | PP of bytes * bytes
+type key = k:CoreCrypto.dh_key{
+  let dhp = k.dh_params in 
+  length dhp.dh_p < 65536 && length dhp.dh_g < 65536 /\
+  length k.dh_public < 65536}
 
-#if 1
-val goodPP_log: FStar.ST.ref (list CoreCrypto.dh_params)
-(* Code should be let goodPP_log = ST.alloc Nil but it misses some type annotations to 
-   compile the OCaml code 
-   TODO : FIXME
-   *)
-let goodPP_log = 
-  let dummy = {
-     dh_p = empty_bytes;
-     dh_g = empty_bytes;
-     dh_q = None;
-     safe_prime = false;
-  } in
-  let nil = Nil in
-  let dummy = dummy::nil in ST.alloc (List.Tot.tl dummy) 
+type group =
+  | Named    of ffdhe
+  | Explicit of params
 
-let goodPP (dhp:dh_params) = List.Tot.mem dhp !goodPP_log
+type secret = bytes
 
-let pp (dhp:CoreCrypto.dh_params) : CoreCrypto.dh_params =
-    goodPP_log := (dhp ::!goodPP_log);
-    dhp
-#endif
+val ffdhe2048: params
+let ffdhe2048 =
+  let p = "ffffffffffffffffadf85458a2bb4a9aafdc5620273d3cf1d8b9c583ce2d3695a9e13641146433fbcc939dce249b3ef97d2fe363630c75d8f681b202aec4617ad3df1ed5d5fd65612433f51f5f066ed0856365553ded1af3b557135e7f57c935984f0c70e0e68b77e2a689daf3efe8721df158a136ade73530acca4f483a797abc0ab182b324fb61d108a94bb2c8e3fbb96adab760d7f4681d4f42a3de394df4ae56ede76372bb190b07a7c8ee0a6d709e02fce1cdf7e2ecc03404cd28342f619172fe9ce98583ff8e4f1232eef28183c3fe3b1b4c6fad733bb5fcbc2ec22005c58ef1837d1683b2c6f34a26c1b2effa886b423861285c97ffffffffffffffff" in
+  let g = "02" in
+  assume (length (bytes_of_hex p) < 65536);
+  assume (length (bytes_of_hex g) < 65536);
+  { 
+    dh_p = bytes_of_hex p;      
+    dh_g = bytes_of_hex g; 
+    dh_q = None;
+    safe_prime = true
+  }
 
+assume val ffdhe3072: params
+assume val ffdhe4096: params
+assume val ffdhe6144: params
+assume val ffdhe8192: params
 
+private val params_of_group: group -> Tot params
+let params_of_group = function
+  | Named FFDHE2048 -> ffdhe2048
+  | Named FFDHE3072 -> ffdhe3072
+  | Named FFDHE4096 -> ffdhe4096
+  | Named FFDHE6144 -> ffdhe6144
+  | Named FFDHE8192 -> ffdhe8192
+  | Explicit params -> params
 
-let genElement dhp: elt =
-    let e = CoreCrypto.dh_gen_key dhp in
-(*
-    assume (Elt(dhp.dhp,dhp.dhg,e));
-*)
-    e.dh_public
+val keygen: group -> Tot key
+let keygen g =
+  let params = params_of_group g in
+  dh_gen_key params
 
-let checkParams dhdb minSize p g =
-    match DHDB.dh_check_params dhdb 
-          DHDB.defaultDHPrimeConfidence 
-          minSize p g with
-    | None -> Error(AD_insufficient_security,"dh_check_params")
-    | Some(res) ->
-        let (dhdb,dhpar) = res in
-#if ideal
-        let dhpar = pp dhpar in
-        let rp = dhpar.dh_p in
-        let rg = dhpar.dh_g in
-        if rp <> p || rg <> g then
-            failwith "Trusted code returned inconsitent value"
-        else
-#endif
-        correct (dhdb,dhpar)
+val dh_responder: key -> Tot (key * secret)
+let dh_responder gx =
+  let params = gx.dh_params in
+  let y = dh_gen_key params in
+  let shared = dh_agreement y gx.dh_public in
+  y, shared
 
+val dh_initiator: key -> key -> Tot secret
+let dh_initiator x gy =
+  dh_agreement x gy.dh_public
 
-let checkElement dhp (b:bytes): option elt =
-    if DHDB.dh_check_element dhp b then
-        (
-(*
-        assume(Elt(dhp.dh_p,dhp.dh_g,b));
-*)
-        Some(b))
-    else
-        None
-
-let defaultDHparams file dhdb minSize =
-    let (dhdb,dhp) = DHDB.load_default_params file dhdb minSize in
-#if ideal
-    let dhp = pp dhp  in
-#endif
-    (dhdb,dhp)
+val serialize: params -> share -> Tot bytes
+let serialize dhp dh_Y =
+  lemma_repr_bytes_values (length (dhp.dh_p));
+  lemma_repr_bytes_values (length (dhp.dh_g));
+  lemma_repr_bytes_values (length dh_Y);
+  let pb  = vlbytes 2 dhp.dh_p in 
+  let gb  = vlbytes 2 dhp.dh_g in
+  let pkb = vlbytes 2 dh_Y in
+  pb @| gb @| pkb
